proof/correctness/MLKEM_keccak_ref.ec
@@ -18,40 +18,381 @@ require import MLKEMFCLib.
 
 from JazzEC require import Jkem WArray200.
 
-(****************************************************************************)
-(****************************************************************************)
-from Keccak require import Keccak1600_ref.
 
-print M.
+(****************************************************************************)
+(****************************************************************************)
+from Keccak require import Keccakf1600_ref Keccak1600_ref.
+
 equiv state_init_ref_eq:
- M(Syscall).__state_init_ref ~ Jazz_avx2.M.__state_init_ref
- : ={arg} ==> ={res}
- by sim.
-
-equiv pstate_init_avx2_eq:
- M(Syscall).__pstate_init_avx2 ~ Jazz_avx2.M.__pstate_init_avx2
+ M(Syscall).__state_init_ref ~ Jazz_ref.M.__state_init_ref
  : ={arg} ==> ={res}
  by sim.
 
 equiv addratebit_avx2_eq:
- M(Syscall).__addratebit_avx2 ~ Jazz_avx2.M.__addratebit_avx2
+ M(Syscall).__addratebit_ref ~ Jazz_ref.M.__addratebit_ref
  : ={arg} ==> ={res}
  by sim.
 
-from JazzEC require import Array1152 Array960 Array128 Array64 Array34 Array33 Array32.
-from JazzEC require import Jkem.
+(****************************************************************************)
+(****************************************************************************)
+from Keccak require import Keccak1600_imem_ref.
 
-axiom sha3_512_33_64 seed : 
- phoare
+equiv absorb_imem_ref_eq:
+ M(Syscall).__absorb_imem_ref ~ Jazz_ref.M.__absorb_imem_ref
+ : ={arg,Glob.mem} ==> ={res,Glob.mem}
+ by sim.
+
+equiv squeeze_imem_ref_eq:
+ M(Syscall).__squeeze_imem_ref ~ Jazz_ref.M.__squeeze_imem_ref
+ : ={arg,Glob.mem} ==> ={res,Glob.mem}
+ by sim.
+
+(****************************************************************************)
+(****************************************************************************)
+from Keccak require Keccak1600_array_ref.
+
+(****************************************************************************)
+from JazzEC require import Array32 WArray32.
+
+clone Keccak1600_array_ref.KeccakArrayRef as A32ref
+ with op aSIZE <- 32,
+      theory A <- Array32,
+      theory WA <- WArray32
+      proof aSIZE_ge0 by done.
+
+equiv a32__squeeze_array_ref_eq:
+ M(Syscall).a32____squeeze_array_ref ~ A32ref.M(A32ref.P).__squeeze_array_ref
+ : ={arg} ==> ={res}
+ by sim.
+
+
+(****************************************************************************)
+from JazzEC require import Array33 WArray33.
+
+clone Keccak1600_array_ref.KeccakArrayRef as A33ref
+ with op aSIZE <- 33,
+      theory A <- Array33,
+      theory WA <- WArray33
+      proof aSIZE_ge0 by done.
+
+equiv a33__absorb_array_ref_eq:
+ M(Syscall).a33____absorb_array_ref ~ A33ref.M(A33ref.P).__absorb_array_ref
+ : ={arg} ==> ={res}
+ by sim.
+
+(****************************************************************************)
+from JazzEC require import Array34 WArray34.
+
+clone Keccak1600_array_ref.KeccakArrayRef as A34ref
+ with op aSIZE <- 34,
+      theory A <- Array34,
+      theory WA <- WArray34
+      proof aSIZE_ge0 by done.
+
+equiv a34__absorb_array_ref_eq:
+ M(Syscall).a34____absorb_array_ref ~ A34ref.M(A34ref.P).__absorb_array_ref
+ : ={arg} ==> ={res}
+ by sim.
+
+(****************************************************************************)
+from JazzEC require import Array64 WArray64.
+
+clone Keccak1600_array_ref.KeccakArrayRef as A64ref
+ with op aSIZE <- 64,
+      theory A <- Array64,
+      theory WA <- WArray64
+      proof aSIZE_ge0 by done.
+
+equiv a64__absorb_array_ref_eq:
+ M(Syscall).a64____absorb_array_ref ~ A64ref.M(A64ref.P).__absorb_array_ref
+ : ={arg} ==> ={res}
+ by sim.
+
+equiv a64__squeeze_array_ref_eq:
+ M(Syscall).a64____squeeze_array_ref ~ A64ref.M(A64ref.P).__squeeze_array_ref
+ : ={arg} ==> ={res}
+ by sim.
+
+(****************************************************************************)
+from JazzEC require import Array128 WArray128.
+
+clone Keccak1600_array_ref.KeccakArrayRef as A128ref
+ with op aSIZE <- 128,
+      theory A <- Array128,
+      theory WA <- WArray128
+      proof aSIZE_ge0 by done.
+
+equiv a128__squeeze_array_ref_eq:
+ M(Syscall).a128____squeeze_array_ref ~ A128ref.M(A128ref.P).__squeeze_array_ref
+ : ={arg} ==> ={res}
+ by sim.
+
+(****************************************************************************)
+from JazzEC require import Array168 WArray168.
+
+clone Keccak1600_array_ref.KeccakArrayRef as A168ref
+ with op aSIZE <- 168,
+      theory A <- Array168,
+      theory WA <- WArray168
+      proof aSIZE_ge0 by done.
+
+equiv a168__dumpstate_array_ref_eq:
+ M(Syscall).a168____dumpstate_array_ref ~ A168ref.M(A168ref.P).__dumpstate_array_ref
+ : ={arg} ==> ={res}
+ by sim.
+
+(****************************************************************************)
+(****************************************************************************)
+
+module K = {
+  proc _shake256_128_33(out : W8.t Array128.t, in_0 : W8.t Array33.t) :
+    W8.t Array128.t = {
+    var st_s : W64.t Array25.t;
+    var st : W64.t Array25.t;
+    var offset : W64.t;
+    var _0 : int;
+    var _1 : W64.t;
+    var _2 : W64.t;
+    var _3 : W64.t Array25.t;
+    
+    _3 <- witness;
+    st <- witness;
+    st_s <- witness;
+    st <- st_s;
+    st <@ Jazz_ref.M.__state_init_ref(st);
+    offset <- W64.zero;
+    (st, _0, _1) <@
+      A33ref.M(A33ref.P).__absorb_array_ref(st, 0, in_0, offset, 33, 136, 31);
+    offset <- W64.zero;
+    (out, _2, _3) <@
+      A128ref.M(A128ref.P).__squeeze_array_ref(out, offset, 128, st, 136);
+    
+    return out;
+  }
+  
+  proc _shake256_1120_32(out : W64.t, in0 : W64.t, in1 : W64.t) : unit = {
+    var st_s : W64.t Array25.t;
+    var st : W64.t Array25.t;
+    var aT : int;
+    var _0 : W64.t;
+    var _1 : int;
+    var _2 : W64.t;
+    var _3 : W64.t;
+    var _4 : W64.t Array25.t;
+    
+    _4 <- witness;
+    st <- witness;
+    st_s <- witness;
+    st <- st_s;
+    st <@ Jazz_ref.M.__state_init_ref(st);
+    (st, _1, _0) <@ Jazz_ref.M.__absorb_imem_ref(st, 0, in0, 32, 136, 0);
+    (st, _1, _2) <@ Jazz_ref.M.__absorb_imem_ref(st, 32, in1, 1088, 136, 31);
+    (_3, _4) <@ Jazz_ref.M.__squeeze_imem_ref(out, 32, st, 136);
+    
+    return tt;
+  }
+  
+  proc _sha3512_33(out : W8.t Array64.t, in_0 : W8.t Array33.t) :
+    W8.t Array64.t = {
+    var st_s : W64.t Array25.t;
+    var st : W64.t Array25.t;
+    var offset : W64.t;
+    var _0 : int;
+    var _1 : W64.t;
+    var _2 : W64.t;
+    var _3 : W64.t Array25.t;
+    
+    _3 <- witness;
+    st <- witness;
+    st_s <- witness;
+    st <- st_s;
+    st <@ Jazz_ref.M.__state_init_ref(st);
+    offset <- W64.zero;
+    (st, _0, _1) <@
+      A33ref.M(A33ref.P).__absorb_array_ref(st, 0, in_0, offset, 33, 72, 6);
+    offset <- W64.zero;
+    (out, _2, _3) <@ A64ref.M(A64ref.P).__squeeze_array_ref(out, offset, 64, st, 72);
+    
+    return out;
+  }
+  
+  proc _shake128_absorb34(st : W64.t Array25.t, in_0 : W8.t Array34.t) :
+    W64.t Array25.t = {
+    var offset : W64.t;
+    var _0 : int;
+    var _1 : W64.t;
+    
+    st <@ Jazz_ref.M.__state_init_ref(st);
+    offset <- W64.zero;
+    (st, _0, _1) <@
+      A34ref.M(A34ref.P).__absorb_array_ref(st, 0, in_0, offset, 34, 168, 31);
+    
+    return st;
+  }
+  
+  proc _shake128_squeezeblock(st : W64.t Array25.t, out : W8.t Array168.t) :
+    W64.t Array25.t * W8.t Array168.t = {
+    var offset : W64.t;
+    var _0 : W64.t;
+    
+    st <@ Jazz_ref.M._keccakf1600_ref(st);
+    offset <- W64.zero;
+    (out, _0) <@ A168ref.M(A168ref.P).__dumpstate_array_ref(out, offset, 168, st);
+    
+    return (st, out);
+  }
+  
+  proc _isha3_256_M1184(out : W8.t Array32.t, in_0 : W64.t) : W8.t Array32.t = {
+    var st_s : W64.t Array25.t;
+    var st : W64.t Array25.t;
+    var offset : W64.t;
+    var _0 : int;
+    var _1 : W64.t;
+    var _2 : W64.t;
+    var _3 : W64.t Array25.t;
+    
+    _3 <- witness;
+    st <- witness;
+    st_s <- witness;
+    st <- st_s;
+    st <@ Jazz_ref.M.__state_init_ref(st);
+    (st, _0, _1) <@ Jazz_ref.M.__absorb_imem_ref(st, 0, in_0, 1184, 136, 6);
+    offset <- W64.zero;
+    (out, _2, _3) <@ A32ref.M(A32ref.P).__squeeze_array_ref(out, offset, 32, st, 136);
+    
+    return out;
+  }
+  
+  proc _sha3_512_64(out : W8.t Array64.t, in_0 : W8.t Array64.t) :
+    W8.t Array64.t = {
+    var st_s : W64.t Array25.t;
+    var st : W64.t Array25.t;
+    var offset : W64.t;
+    var _0 : int;
+    var _1 : W64.t;
+    var _2 : W64.t;
+    var _3 : W64.t Array25.t;
+    
+    _3 <- witness;
+    st <- witness;
+    st_s <- witness;
+    st <- st_s;
+    st <@ Jazz_ref.M.__state_init_ref(st);
+    offset <- W64.zero;
+    (st, _0, _1) <@
+      A64ref.M(A64ref.P).__absorb_array_ref(st, 0, in_0, offset, 64, 72, 6);
+    offset <- W64.zero;
+    (out, _2, _3) <@ A64ref.M(A64ref.P).__squeeze_array_ref(out, offset, 64, st, 72);
+    
+    return out;
+  }
+}.
+
+
+(****************************************************************************)
+(****************************************************************************)
+from JazzEC require import Array1152 Array960.
+
+
+(****************************************************************************)
+equiv sha3512_33_eq:
+  M(Syscall)._sha3512_33 ~ K._sha3512_33
+ : ={arg} ==> ={res}
+by sim.
+
+hoare sha3512_33_h' seed : 
+ K._sha3512_33
+ : arg.`2 = seed
+ ==>
+    Array32.init (fun i => res.[i]) = (SHA3_512_33_64 seed).`1
+ /\ Array32.init(fun i => res.[32 + i]) = (SHA3_512_33_64 seed).`2.
+proof.
+proc.
+ecall (A64ref.squeeze_array_ref_h out offset 64 st 72) => /=.
+wp; ecall (A33ref.absorb_array_ref_h [<:W8.t>] in_0 offset 33 72 6).
+wp; ecall (state_init_ref_h 72).
+auto => /> &m []st2 ?? /= -> ?.
+move=> []out?st1 /= Eout ??; rewrite /SHA3_512_33_64 /=.
+have EEout: out = Array64.of_list W8.zero (SHA3_512 (to_list seed)).
+ rewrite Eout tP => i Hi.
+ rewrite filliE 1:/# Hi /= get_of_list 1://; congr.
+ rewrite /SHA3_512 /KECCAK1600; congr; 1:smt(); congr; 1..2:smt().
+ by apply eq_in_mkseq => k Hk.
+split; rewrite tP => i Hi.
+ by rewrite initiE 1:// get_of_list 1:// nth_take 1..2:/# EEout get_of_list /#.
+by rewrite initiE 1:// get_of_list 1:// nth_drop 1..2:/# EEout /= get_of_list /#.
+qed.
+
+lemma sha3512_33_ll: islossless K._sha3512_33.
+proof.
+proc.
+call A64ref.squeeze_array_ref_ll.
+wp; call A33ref.absorb_array_ref_ll.
+wp; call state_init_ref_ll.
+by auto.
+qed.
+
+phoare sha3512_33_ph' seed : 
+ [ K._sha3512_33
+ : arg.`2 = seed
+ ==>
+    Array32.init (fun i => res.[i]) = (SHA3_512_33_64 seed).`1
+ /\ Array32.init(fun i => res.[32 + i]) = (SHA3_512_33_64 seed).`2
+ ] = 1%r.
+proof. by conseq sha3512_33_ll (sha3512_33_h' seed). qed.
+
+phoare sha3_512_33_64 seed : 
  [ Jkem.M(Jkem.Syscall)._sha3512_33
  : arg.`2 = seed
  ==>
    Array32.init (fun i => res.[i]) = (SHA3_512_33_64 seed).`1
  /\ Array32.init(fun i => res.[32 + i]) = (SHA3_512_33_64 seed).`2
  ] = 1%r.
+proof. by conseq sha3512_33_eq (sha3512_33_ph' seed) => /> /#. qed.
 
-axiom shake_absorb (seed : W8.t Array34.t): 
- phoare
+(****************************************************************************)
+equiv shake128_absorb34_eq:
+  M(Syscall)._shake128_absorb34 ~ K._shake128_absorb34
+ : ={arg} ==> ={res}
+by sim.
+
+hoare shake128_absorb34_h' (seed : W8.t Array34.t): 
+ K._shake128_absorb34
+ : arg.`2 = seed
+ ==> res = SHAKE128_ABSORB_34 
+            (Array32.init (fun k => seed.[k]))
+            (seed.[32])
+            (seed.[33]).
+proof.
+proc.
+ecall (A34ref.absorb_array_ref_h [<:W8.t>] in_0 offset 34 168 31).
+wp; ecall (state_init_ref_h 168).
+auto => /> []st1 ?? /= -> ?.
+rewrite /SHAKE128_ABSORB_34; congr; 1..2:smt().
+rewrite /sub (:34=32+2) 1:// mkseq_add 1..2://; congr.
+ by apply eq_in_mkseq => i Hi /=; rewrite initiE /#.
+by rewrite /mkseq -iotaredE /=.
+qed.
+
+lemma shake128_absorb34_ll: islossless K._shake128_absorb34.
+proof.
+proc.
+call A34ref.absorb_array_ref_ll.
+wp; call state_init_ref_ll.
+by auto.
+qed.
+
+phoare shake128_absorb34_ph' (seed : W8.t Array34.t): 
+ [ K._shake128_absorb34
+ : arg.`2 = seed
+ ==> res = SHAKE128_ABSORB_34 
+            (Array32.init (fun k => seed.[k]))
+            (seed.[32])
+            (seed.[33])
+ ] = 1%r.
+proof. by conseq shake128_absorb34_ll (shake128_absorb34_h' seed). qed.
+
+phoare shake_absorb (seed : W8.t Array34.t): 
  [ Jkem.M(Jkem.Syscall)._shake128_absorb34
  : arg.`2 = seed
  ==> res = SHAKE128_ABSORB_34 
@@ -59,31 +400,160 @@ axiom shake_absorb (seed : W8.t Array34.t):
             (seed.[32])
             (seed.[33])
  ] = 1%r.
+proof. by conseq shake128_absorb34_eq (shake128_absorb34_ph' seed) => /> /#. qed.
 
-axiom shake_squeeze state : 
- phoare
+(****************************************************************************)
+equiv shake128_squeezeblock_eq:
+  M(Syscall)._shake128_squeezeblock ~ K._shake128_squeezeblock
+ : ={arg} ==> ={res}
+by sim.
+
+hoare shake128_squeezeblock_h' state : 
+ K._shake128_squeezeblock
+ : arg.`1 = state
+ ==> res = SHAKE128_SQUEEZE_168 state.
+proof.
+proc.
+ecall (A168ref.dumpstate_array_ref_h out offset 168 st).
+wp; ecall (keccakf1600_ref_h st).
+auto => /> &m []st1 ? /= @/SHAKE128_SQUEEZE_168 -> ? /=; split.
+ by rewrite /st_i iter1.
+rewrite tP => i Hi; rewrite filliE 1:// Hi get_of_list //=.
+by rewrite /squeezestate_i /st_i iter1 /squeezestate nth_take 1..2:/# state2bytesE.
+qed.
+
+lemma shake128_squeezeblock_ll: islossless K._shake128_squeezeblock.
+proof.
+proc.
+call A168ref.dumpstate_array_ref_ll.
+wp; call keccakf1600_ref_ll.
+by auto.
+qed.
+
+phoare shake128_squeezeblock_ph' state : 
+ [ K._shake128_squeezeblock
+ : arg.`1 = state
+ ==> res = SHAKE128_SQUEEZE_168 state
+ ] = 1%r.
+proof. by conseq shake128_squeezeblock_ll (shake128_squeezeblock_h' state). qed.
+
+phoare shake_squeeze state : 
  [ Jkem.M(Jkem.Syscall)._shake128_squeezeblock
  : arg.`1 = state
  ==> res = SHAKE128_SQUEEZE_168 state
  ] = 1%r.
+proof. by conseq shake128_squeezeblock_eq (shake128_squeezeblock_ph' state) => /> /#. qed.
 
-axiom shake256_33_128 seed : 
- phoare
+(****************************************************************************)
+equiv shake256_128_33_eq:
+  M(Syscall)._shake256_128_33 ~ K._shake256_128_33
+ : ={arg} ==> ={res}
+by sim.
+
+hoare shake256_128_33_h' seed : 
+ K._shake256_128_33
+ : arg.`2 = seed
+ ==> res = SHAKE256_33_128
+            (Array32.init (fun i => seed.[i]))
+            seed.[32].
+proof.
+proc.
+ecall (A128ref.squeeze_array_ref_h out offset 128 st 136).
+wp; ecall (A33ref.absorb_array_ref_h [<:W8.t>] in_0 offset 33 136 31).
+wp; call (state_init_ref_h 136).
+auto => /> &m []st1 ?? /= ->?.
+move=> []out ? ? /= -> ??.
+rewrite tP=> i Hi; rewrite filliE 1:/# Hi /SHAKE256_33_128 get_of_list 1:/# /=.
+congr; rewrite /SHAKE256 /KECCAK1600; congr; 1:smt().
+congr; 1..2:smt().
+rewrite /sub (:33=32+1) 1:// mkseq_add 1..2://; congr.
+ by apply eq_in_mkseq => k Hk /=; rewrite initiE /#.
+by rewrite /mkseq -iotaredE /=.
+qed.
+
+lemma shake256_128_33_ll: islossless K._shake256_128_33.
+proof.
+proc.
+call A128ref.squeeze_array_ref_ll.
+wp; call A33ref.absorb_array_ref_ll.
+wp; call state_init_ref_ll.
+by auto.
+qed.
+
+phoare shake256_128_33_ph' seed : 
+ [ K._shake256_128_33
+ : arg.`2 = seed
+ ==> res = SHAKE256_33_128
+            (Array32.init (fun i => seed.[i]))
+            seed.[32]
+ ] = 1%r.
+proof. by conseq shake256_128_33_ll (shake256_128_33_h' seed). qed.
+
+phoare shake256_33_128 seed : 
  [ Jkem.M(Jkem.Syscall)._shake256_128_33
  : arg.`2 = seed
  ==> res = SHAKE256_33_128
             (Array32.init (fun i => seed.[i]))
             seed.[32]
  ] = 1%r.
+proof. by conseq shake256_128_33_eq (shake256_128_33_ph' seed) => /> /#. qed.
 
-axiom shake256_33_128_ll:
- islossless M(Syscall)._shake256_128_33.
+lemma shake256_33_128_ll: islossless M(Syscall)._shake256_128_33.
+proof. by conseq shake256_128_33_eq shake256_128_33_ll => /> /#. qed.
 
-axiom pkH_sha mem _ptr: 
- phoare
- [ Jkem.M(Jkem.Syscall)._isha3_256
+(****************************************************************************)
+equiv isha3_256_M1184_eq:
+  M(Syscall)._isha3_256_M1184 ~ K._isha3_256_M1184
+ : ={arg, Glob.mem} ==> ={res, Glob.mem}
+ by sim.
+
+hoare isha3_256_M1184_h' _mem _ptr: 
+ K._isha3_256_M1184
  : arg.`2 = W64.of_int _ptr
- /\ arg.`3 = W64.of_int (3*384+32)
+ /\ valid_ptr _ptr 1184
+ /\ Glob.mem = _mem
+ ==> Glob.mem = _mem
+  /\ res = SHA3_256_1184_32
+            (Array1152.init (fun k => _mem.[_ptr+k]),
+             Array32.init (fun k => _mem.[_ptr+1152+k])).
+proof.
+proc.
+ecall (A32ref.squeeze_array_ref_h out offset 32 st 136).
+wp; ecall (absorb_imem_ref_h [<:W8.t>] _mem in_0 1184 136 6).
+call (state_init_ref_h 136).
+auto => /> &m Hp1 Hp2; rewrite !of_uintK; split; first smt().
+move => _ []st ?? /= -> ?.
+move=> []out ?? -> /= ??; rewrite tP => i Hi.
+rewrite filliE 1:// Hi /SHA3_256_1184_32 get_of_list 1:// /=.
+rewrite /SHA3_256 /KECCAK1600; congr; congr; 1:smt(); congr; 1..2:smt().
+rewrite /memread (:1184=1152+32) 1:// mkseq_add 1..2://; congr.
+ by apply eq_in_mkseq => k Hk /=; rewrite initiE /#.
+by apply eq_in_mkseq => k Hk /=; rewrite initiE /#.
+qed.
+
+lemma isha3_256_M1184_ll: islossless K._isha3_256_M1184.
+proc.
+call A32ref.squeeze_array_ref_ll.
+wp; call absorb_imem_ref_ll.
+wp; call state_init_ref_ll.
+by auto.
+qed.
+
+phoare isha3_256_M1184_ph' _mem _ptr: 
+ [ K._isha3_256_M1184
+ : arg.`2 = W64.of_int _ptr
+ /\ valid_ptr _ptr 1184
+ /\ Glob.mem = _mem
+ ==> Glob.mem = _mem
+  /\ res = SHA3_256_1184_32
+            (Array1152.init (fun k => _mem.[_ptr+k]),
+             Array32.init (fun k => _mem.[_ptr+1152+k]))
+ ] = 1%r.
+proof. by conseq isha3_256_M1184_ll (isha3_256_M1184_h' _mem _ptr). qed.
+
+phoare pkH_sha mem _ptr: 
+ [ Jkem.M(Jkem.Syscall)._isha3_256_M1184
+ : arg.`2 = W64.of_int _ptr
  /\ valid_ptr _ptr 1184
  /\ Glob.mem = mem
  ==> Glob.mem = mem
@@ -91,9 +561,78 @@ axiom pkH_sha mem _ptr:
             (Array1152.init (fun k => mem.[_ptr+k]),
              Array32.init (fun k => mem.[_ptr+1152+k]))
  ] = 1%r.
+proof. by conseq isha3_256_M1184_eq (isha3_256_M1184_ph' mem _ptr) => /> /#. qed.
 
-axiom j_shake mem _pout _pin1 _pin2: 
- phoare
+(****************************************************************************)
+equiv shake256_1120_32_eq:
+  M(Syscall)._shake256_1120_32 ~ K._shake256_1120_32
+ : ={arg, Glob.mem} ==> ={res, Glob.mem}
+ by sim.
+
+hoare shake256_1120_32_h' mem _pout _pin1 _pin2: 
+ K._shake256_1120_32
+ : arg = (W64.of_int _pout,W64.of_int _pin1,W64.of_int _pin2)
+ /\ valid_ptr _pout 32
+ /\ valid_ptr _pin1 32
+ /\ valid_ptr _pin2 1088
+ /\ Glob.mem = mem
+ ==> touches Glob.mem mem _pout 32
+  /\ Array32.init (fun k => Glob.mem.[_pout+k])
+     = SHAKE_256_1120_32
+        (Array32.init (fun k => mem.[_pin1+k])) 
+        ( Array960.init (fun k => mem.[_pin2+k])
+        , Array128.init (fun k => mem.[_pin2+960+k])).
+proof.
+proc.
+ecall (squeeze_imem_ref_h Glob.mem out 32 st 136).
+ecall (absorb_imem_ref_h (memread mem _pin1 32) Glob.mem in1 1088 136 31).
+ecall (absorb_imem_ref_h [<:W8.t>] Glob.mem in0 32 136 0).
+call (state_init_ref_h 136).
+auto; rewrite /valid_ptr => |> ??????; rewrite !of_uintK.
+move=> st1 H1; split; first smt().
+move=> _ []st2 ?? /= ? ??; split.
+ by rewrite size_memread /#.
+move=> _ H2 ? [] st3 ? /= out -> _; split; first smt().
+move=> _ []?? /= _ _.
+split.
+ by rewrite /touches => i Hi; rewrite get_storesE size_SQUEEZE1600 1..2:// ifF /#.
+rewrite /SHAKE_256_1120_32 tP => i Hi /=; rewrite initiE 1:// get_of_list 1:// /=.
+rewrite get_storesE size_SQUEEZE1600 1..2:// ifT 1:/# /SHAKE256 /KECCAK1600; congr; 2:smt().
+congr; 1:smt(); congr; 1..2:smt().
+rewrite -catA; congr.
+ by apply eq_in_mkseq => k Hk /=; rewrite initiE /#.
+rewrite /memread (:1088=960+128) 1:// mkseq_add 1..2://; congr.
+ by apply eq_in_mkseq => k Hk /=; rewrite initiE /#.
+by apply eq_in_mkseq => k Hk /=; rewrite initiE /#.
+qed.
+
+lemma shake256_1120_32_ll: islossless K._shake256_1120_32.
+proof.
+proc.
+call squeeze_imem_ref_ll => /=.
+call absorb_imem_ref_ll.
+call absorb_imem_ref_ll.
+call state_init_ref_ll.
+by auto => />.
+qed.
+
+phoare shake256_1120_32_ph' mem _pout _pin1 _pin2: 
+ [ K._shake256_1120_32
+ : arg = (W64.of_int _pout,W64.of_int _pin1,W64.of_int _pin2)
+ /\ valid_ptr _pout 32
+ /\ valid_ptr _pin1 32
+ /\ valid_ptr _pin2 1088
+ /\ Glob.mem = mem
+ ==> touches Glob.mem mem _pout 32
+  /\ Array32.init (fun k => Glob.mem.[_pout+k])
+     = SHAKE_256_1120_32
+        (Array32.init (fun k => mem.[_pin1+k])) 
+        ( Array960.init (fun k => mem.[_pin2+k])
+        , Array128.init (fun k => mem.[_pin2+960+k]))
+ ] = 1%r.
+proof. by conseq shake256_1120_32_ll (shake256_1120_32_h' mem _pout _pin1 _pin2). qed.
+
+phoare j_shake mem _pout _pin1 _pin2: 
  [ Jkem.M(Syscall)._shake256_1120_32
  : arg = (W64.of_int _pout,W64.of_int _pin1,W64.of_int _pin2)
  /\ valid_ptr _pout 32
@@ -107,9 +646,71 @@ axiom j_shake mem _pout _pin1 _pin2:
         ( Array960.init (fun k => mem.[_pin2+k])
         , Array128.init (fun k => mem.[_pin2+960+k]))
  ] = 1%r.
+proof. by conseq shake256_1120_32_eq (shake256_1120_32_ph' mem _pout _pin1 _pin2) => /> /#. qed.
 
-axiom sha_g buf: 
- phoare
+(****************************************************************************)
+equiv sha3_512_64_eq:
+  M(Syscall)._sha3_512_64 ~ K._sha3_512_64
+ : ={arg} ==> ={res}
+ by sim.
+
+hoare sha3_512_64_h' buf:
+ K._sha3_512_64
+ : arg.`2 = buf
+ ==>
+   let bytes = SHA3_512_64_64
+                (Array32.init (fun k => buf.[k]))
+                (Array32.init (fun k => buf.[k+32]))
+   in res = Array64.init
+             (fun k => if k < 32
+                       then bytes.`1.[k]
+                       else bytes.`2.[k-32]).
+proof.
+proc.
+ecall (A64ref.squeeze_array_ref_h out offset 64 st 72).
+wp; ecall (A64ref.absorb_array_ref_h [<:W8.t>] in_0 offset 64 72 6).
+wp; call (state_init_ref_h 72).
+auto => /> &m []st1 ?? /= ->?.
+move=> []out ? ? /= -> ??.
+rewrite tP=> i Hi; rewrite filliE 1:/# Hi /SHA3_512_64_64 initiE 1:/# /=.
+rewrite /SHA3_512 /KECCAK1600; case:(i<32) =>C.
+ rewrite get_of_list 1:/# !nth_take 1..6:/# /=; congr; congr; 1:smt().
+ congr; 1..2:smt().
+  rewrite /sub (:64=32+32) 1:// mkseq_add 1..2:/#; congr.
+   by apply eq_in_mkseq => k Hk /=; rewrite initiE /#.
+  by apply eq_in_mkseq => k Hk /=; rewrite initiE /#.
+ smt().
+rewrite get_of_list 1:/# !nth_drop 1..2:/# /=; congr; congr; 1:smt().
+congr; 1..2:smt().
+rewrite /sub (:64=32+32) 1:// mkseq_add 1..2:/#; congr.
+ by apply eq_in_mkseq => k Hk /=; rewrite initiE /#.
+by apply eq_in_mkseq => k Hk /=; rewrite initiE /#.
+qed.
+
+lemma sha3_512_64_ll: islossless K._sha3_512_64.
+proof.
+proc.
+call A64ref.squeeze_array_ref_ll.
+wp; call A64ref.absorb_array_ref_ll.
+wp; call state_init_ref_ll.
+by auto.
+qed.
+
+phoare sha3_512_64_ph' buf:
+ [ K._sha3_512_64
+ : arg.`2 = buf
+ ==>
+   let bytes = SHA3_512_64_64
+                (Array32.init (fun k => buf.[k]))
+                (Array32.init (fun k => buf.[k+32]))
+   in res = Array64.init
+             (fun k => if k < 32
+                       then bytes.`1.[k]
+                       else bytes.`2.[k-32])
+ ] = 1%r.
+proof. by conseq sha3_512_64_ll (sha3_512_64_h' buf). qed.
+
+phoare sha_g buf: 
  [ Jkem.M(Jkem.Syscall)._sha3_512_64
  : arg.`2 = buf
  ==>
@@ -121,5 +722,4 @@ axiom sha_g buf:
                        then bytes.`1.[k]
                        else bytes.`2.[k-32])
  ] = 1%r.
-
-
+proof. by conseq sha3_512_64_eq (sha3_512_64_ph' buf) => /> /#. qed.
